architectures.v
@@ -2,10 +2,9 @@
 (* This file is distributed under the terms of the BSD license. *)
 Require Export architecture_spec.
 
-Definition x86 : architecture.
+Definition ilp32 : architecture_sizes.
 Proof.
  refine {|
-  arch_big_endian := false;
   arch_char_bits := 8;
   arch_size k :=
     match k with
@@ -15,16 +14,17 @@ Proof.
   arch_align k :=
     match k with
     | CharRank => 1 | ShortRank => 2 | IntRank | LongRank => 4
-    | LongLongRank => 4
+    | LongLongRank => 8
     end;
   arch_ptr_rank := LongRank
  |}; by apply (bool_decide_unpack _); vm_compute.
 Defined.
 
-Definition x86_64 : architecture.
+(** See http://en.wikipedia.org/wiki/64-bit_computing#64-bit_data_models *)
+(** LLP64 is used by Microsoft Windows (x86-64 and IA-64) *)
+Definition llp64 : architecture_sizes.
 Proof.
  refine {|
-  arch_big_endian := false;
   arch_char_bits := 8;
   arch_size k :=
     match k with
@@ -36,14 +36,15 @@ Proof.
     | CharRank => 1 | ShortRank => 2 | IntRank => 4
     | LongRank | LongLongRank => 8
     end;
-  arch_ptr_rank := LongRank
+  arch_ptr_rank := LongLongRank
  |}; by apply (bool_decide_unpack _); vm_compute.
 Defined.
 
-Definition arm : architecture.
+(** LP64 is used by most Unix and Unix-like systems, e.g. Solaris, Linux, BSD,
+and OS X; z/OS *)
+Definition lp64 : architecture_sizes.
 Proof.
  refine {|
-  arch_big_endian := false;
   arch_char_bits := 8;
   arch_size k :=
     match k with
@@ -55,25 +56,6 @@ Proof.
     | CharRank => 1 | ShortRank => 2 | IntRank | LongRank => 4
     | LongLongRank => 8
     end;
-  arch_ptr_rank := LongRank
- |}; by apply (bool_decide_unpack _); vm_compute.
-Defined.
-
-Definition ppc : architecture.
-Proof.
- refine {|
-  arch_big_endian := true;
-  arch_char_bits := 8;
-  arch_size k :=
-    match k with
-    | CharRank => 1 | ShortRank => 2 | IntRank | LongRank => 4
-    | LongLongRank => 8
-    end;
-  arch_align k :=
-    match k with
-    | CharRank => 1 | ShortRank => 2 | IntRank | LongRank => 4
-    | LongLongRank => 8
-    end;
-  arch_ptr_rank := LongRank
+  arch_ptr_rank := LongLongRank
  |}; by apply (bool_decide_unpack _); vm_compute.
 Defined.
